demo/fib/Fib34proof.v
@@ -1,0 +1,441 @@
+Require Import CoqlibC Maps Postorder.
+Require Import AST Linking.
+Require Import ValuesC MemoryC GlobalenvsC Events Smallstep.
+Require Import Op ClightC.
+Require Import CtypesC CtypingC.
+Require Import sflib.
+Require Import IntegersC.
+
+Require Import Simulation.
+Require Import Skeleton Mod ModSem SimMod SimModSemLift SimSymb SimMemLift MatchSimModSemExcl.
+Require SoundTop.
+Require SimMemId.
+Require Import Any.
+Require Import SIRmini.
+Require Import SIRmini_stack.
+Require Import Fib4.
+Require Import Fib3.
+Require Import ModSemProps.
+Require Import Program.
+Require Import SIRProps.
+
+Set Implicit Arguments.
+
+
+
+
+
+
+
+
+
+Lemma bind_unwrapU
+      E `{EventE -< E} R S
+      (r: option R) r'
+      (k: R -> itree E S)
+      (SOME: r = Some r')
+  :
+    ` x : _ <- unwrapU r;; k x = k r'.
+Proof.
+  rewrite SOME. cbn. eapply bind_ret_l.
+Qed.
+
+Lemma bind_unwrapN
+      E `{EventE -< E} R S
+      (r: option R) r'
+      (k: R -> itree E S)
+      (SOME: r = Some r')
+  :
+    ` x : _ <- unwrapN r;; k x = k r'.
+Proof.
+  rewrite SOME. cbn. eapply bind_ret_l.
+Qed.
+
+Lemma bind_bind : forall (E : Type -> Type) (R S T : Type) (s : itree E R) (k : R -> itree E S) (h : S -> itree E T),
+    ` x : _ <- (` x : _ <- s;; k x);; h x = ` r : R <- s;; ` x : _ <- k r;; h x.
+Proof.
+  i. f. eapply bind_bind.
+Qed.
+
+Lemma bind_assume
+      E `{EventE -< E} R
+      (P: Prop)
+      (prf: P)
+      (k: itree E R)
+  :
+    assume P ;; k = k.
+Proof.
+  unfold assume. des_ifs. rewrite bind_ret_l. ss.
+Qed.
+
+Lemma bind_guarantee
+      E `{EventE -< E} R
+      (P: Prop)
+      (prf: P)
+      (k: itree E R)
+  :
+    guarantee P ;; k = k.
+Proof.
+  unfold guarantee. des_ifs. rewrite bind_ret_l. ss.
+Qed.
+
+Lemma interp_mrec_bind :
+forall (D E : Type -> Type) (ctx : forall T : Type, D T -> itree (D +' E) T) (U T : Type) (t : itree (D +' E) U)
+  (k : U -> itree (D +' E) T), interp_mrec ctx (` x : _ <- t;; k x) = ` x : U <- interp_mrec ctx t;; interp_mrec ctx (k x).
+Proof. i. f. eapply interp_mrec_bind. Qed.
+
+
+
+
+
+
+
+
+
+
+
+Lemma eta
+      i j
+      (EQ: i.(Int.intval) = j.(Int.intval))
+  :
+    <<EQ: i = j>>
+.
+Proof.
+  r. destruct i, j; ss. clarify. f_equal. eapply Axioms.proof_irr.
+Qed.
+
+(* Lemma signed_inj *)
+(*       i j *)
+(*       (EQ: Int.signed i = Int.signed j) *)
+(*   : *)
+(*     <<EQ: i = j>> *)
+(* . *)
+(* Proof. *)
+(*   unfold Int.signed in *. des_ifs. *)
+(*   - r. eapply eta. ss. *)
+(*   - r. eapply eta. ss. *)
+(* Qed. *)
+
+Lemma Int_add_repr: forall x y,
+    <<EQ: (Int.add (Int.repr x) (Int.repr y)) = Int.repr (x + y)>>.
+Proof.
+  i. apply Int.eqm_repr_eq. eapply Int.eqm_sym. eapply Int.eqm_trans.
+  - apply Int.eqm_sym. apply Int.eqm_unsigned_repr.
+  - apply Int.eqm_add; apply Int.eqm_unsigned_repr.
+Qed.
+
+Lemma Int_sub_repr: forall x y,
+    <<EQ: (Int.sub (Int.repr x) (Int.repr y)) = Int.repr (x - y)>>.
+Proof.
+  i. apply Int.eqm_repr_eq. eapply Int.eqm_sym. eapply Int.eqm_trans.
+  - apply Int.eqm_sym. apply Int.eqm_unsigned_repr.
+  - apply Int.eqm_sub; apply Int.eqm_unsigned_repr.
+Qed.
+
+Lemma bind_trigger: forall (E : Type -> Type) (R U : Type) (e : E U) (k : U -> itree E R),
+    ` x : _ <- ITree.trigger e;; k x = Vis e (fun x : U => k x).
+Proof. i. f. eapply bind_trigger. Qed.
+
+Local Opaque ident_eq.
+Local Opaque Z.of_nat.
+
+Ltac step := gstep; econs; et.
+Definition mp: ModPair.t := SimSymbId.mk_mp (Fib4.module) (Fib3.module).
+
+(* Hint Unfold assume guarantee assumeK guaranteeK triggerUB triggerNB unwrapU unwrapN. *)
+Hint Unfold of_nat to_nat of_nat_opt to_nat_opt.
+
+Lemma fib_nat_0: (fib_nat 0 = 0)%nat. Proof. ss. Qed.
+Lemma fib_nat_1: (fib_nat 1 = 1)%nat. Proof. ss. Qed.
+Lemma fib_nat_recurse: forall n, ((fib_nat (S (S n))) = (fib_nat n) + fib_nat (S n))%nat.
+Proof. reflexivity. Qed.
+Local Opaque fib_nat.
+
+Theorem sim_mod: ModPair.sim mp.
+Proof.
+  assert(tau: forall E R (a: itree E R), (tau;; a) = a).
+  { admit "backdoor". }
+  assert(forall fname oh0 m0 vs0, sim_st eq (interp_program0 Fib4.prog (ICall fname oh0 m0 vs0))
+                                         (interp_program0 prog (ICall fname oh0 m0 vs0))).
+  {
+    ginit.
+    { i. eapply cpn2_wcompat; eauto with paco. }
+    ii.
+    unfold interp_program0, mrec. ss.
+    destruct(ident_eq fname Fib0._fib); cycle 1.
+    {
+      unfold Fib4.prog, prog. ss. des_ifs.
+      unfold sim_st. unfold triggerNB.
+      rewrite ! unfold_interp_mrec. cbn. step.
+    }
+    des_ifs.
+    set (interp_function Fib4.prog) as X.
+    set (interp_function prog) as Y.
+    unfold Fib4.prog, prog in *. ss. des_ifs.
+    unfold Fib4.f_fib, f_fib. ss.
+    replace Fib4.precond with precond; ss.
+    replace Fib4.fib_nat with fib_nat; ss.
+    destruct (precond vs0) eqn:T; cycle 1.
+    { rewrite ! unfold_interp_mrec. cbn. step.
+      rewrite ! unfold_interp_mrec. cbn. step.
+    }
+    clear T vs0.
+    (* https://coq-club.inria.narkive.com/VWS50VZQ/adding-strong-induction-to-the-standard-library *)
+    induction n as [ n IHn ] using (well_founded_induction lt_wf); ii; ss.
+    destruct n eqn:U0.
+    { rewrite ! unfold_interp_mrec. cbn. step.
+      rewrite ! bind_ret_l.
+      unfold guaranteeK. des_ifs; cycle 1.
+      { unfold NW in *. repeat (Psimpl; des; ss). }
+      des; clarify. ss. rewrite V. clear_tac.
+      rewrite ! unfold_interp_mrec. cbn. rewrite tau. unfold Fib4.of_nat.
+      rewrite ! unfold_interp_mrec. cbn. rewrite tau.
+      rewrite ! unfold_interp_mrec. cbn.
+      step.
+    }
+    destruct n0 eqn:U1.
+    { rewrite ! unfold_interp_mrec. cbn. step.
+      rewrite ! bind_ret_l.
+      unfold guaranteeK. des_ifs; cycle 1.
+      { unfold NW in *. repeat (Psimpl; des; ss). }
+      des; clarify. ss. rewrite V. clear_tac.
+      rewrite ! unfold_interp_mrec. cbn. rewrite tau. unfold Fib4.of_nat.
+      rewrite ! unfold_interp_mrec. cbn. rewrite tau.
+      rewrite ! unfold_interp_mrec. cbn.
+      step.
+    }
+    rewrite ! unfold_interp_mrec. cbn. step.
+    rewrite ! bind_ret_l.
+    rewrite ! tau.
+    Ltac step_unwrapN := match goal with
+                         | |- context[unwrapN ?ox ;; _] =>
+                           (*** I want to unfold only the "first" assume.
+Maybe we should use notation instead, so that we can avoid this weird "unfold"? ***)
+                           first[
+                               unfold unwrapN at 5|
+                               unfold unwrapN at 4|
+                               unfold unwrapN at 3|
+                               unfold unwrapN at 2|
+                               unfold unwrapN at 1|
+                               unfold unwrapN at 0
+                             ];
+                           let name := fresh "T" in
+                           destruct ox eqn:name; cycle 1
+                         end
+    .
+    step_unwrapN.
+    { rewrite ! unfold_interp_mrec. cbn. step. }
+    cbn. rewrite bind_ret_l.
+    rewrite bind_bind.
+    rewrite ! unfold_interp_mrec. cbn. rewrite ! tau.
+    exploit (IHn n0); eauto.
+    { xomega. }
+    intro V. repeat (rewrite ! tau in *; rewrite bind_ret_l in *).
+    rewrite interp_mrec_trigger.
+    step.
+
+    rewrite ! unfold_interp_mrec. cbn. step.
+    unfold guaranteeK. des_ifs; cycle 1.
+    { unfold NW in *. repeat (Psimpl; des; ss). }
+    des; clarify. ss. rewrite V. clear_tac.
+    rewrite ! unfold_interp_mrec. cbn. rewrite tau. unfold Fib4.of_nat.
+    rewrite ! unfold_interp_mrec. cbn. rewrite tau.
+    rewrite ! unfold_interp_mrec. cbn.
+    step.
+    
+    {
+      rewrite ! unfold_interp_mrec.
+    }
+    assert(precond vs0 = Some n).
+    unfold Fib4.f_fib, f_fib.
+    rewrite ! unfold_interp_mrec. ss. cbn. step.
+    rewrite 
+    cbn.
+      cecons; et.
+        eapply sim_st_nb. econs; et.
+        rewrite <- ! bind_trigger. rewrite ! interp_mrec_bind.
+      eapply sim_st_nb. econs; et.
+      step.
+      econs; et.
+    }
+    unfold interp_program0. ss.
+  }
+  assert(Fib4.module = Fib3.module).
+  {
+    unfold Fib4.module. unfold module. f_equal.
+    unfold Fib4.prog. unfold prog. f_equal.
+    apply func_ext3. intros oh0 m0 vs0.
+                                           (Fib4.f_fib oh0 m0 vs0) (f_fib oh0 m0 vs0)).
+    unfold Fib4.f_fib. unfold f_fib.
+    f.
+    do 2 f_equiv. replace Fib4.precond with precond; ss.
+    f_equiv. ii.
+    f.
+    assert(tau: forall (a: itree (E owned_heap) (owned_heap * (mem * val))), (tau;; a) = a).
+    { admit "backdoor". }
+    induction a; ii; ss.
+    - rewrite ! tau.
+      rewrite bind_ret_l. unfold guaranteeK. des_ifs.
+    do 2 f_equiv. ii.
+    econs; et.
+    f_equal.
+  }
+  eapply SimSIR.sim_mod with (SO := eq); ss.
+  ii. clarify. unfold Fib3.prog, prog. ss. des_ifs; econs; et.
+  ii. clarify. unfold Fib3.owned_heap in *. des_u. ss.
+  revert m vs.
+  ginit.
+  { i. eapply cpn2_wcompat; eauto with paco. }
+  gcofix CIH. ii.
+  step.
+  destruct (precond vs) eqn:T; cycle 1.
+  { cbn. unfold triggerUB. rewrite bind_vis. step. }
+  cbn. rewrite bind_ret_l. unfold precond in *. des_ifs_safe. unfold to_nat_opt in T. set n as x. des_ifs_safe.
+  destruct x eqn:T.
+  { rewrite bind_ret_l. u. rewrite fib_nat_0. unfold guaranteeK. cbn.
+    rewrite Nat2Z.inj_0. fold Int.zero.
+    assert(i = Int.zero).
+    { subst x.
+      assert((Int.signed i) = 0).
+      { apply Z2Nat.inj; ss. }
+      apply func_app with (f:=Int.repr) in H. rewrite Int.repr_signed in H. ss.
+    }
+    clarify.
+    rewrite Int.eq_true. des_ifs; repeat (Psimpl; des; ss; et).
+    step.
+  }
+  destruct n eqn:U.
+  { rewrite bind_ret_l. u. rewrite fib_nat_1. unfold guaranteeK. cbn.
+    rewrite Nat2Z.inj_succ. rewrite Nat2Z.inj_0. cbn. fold Int.one.
+    assert(i = Int.one).
+    { subst x.
+      assert((Int.signed i) = 1).
+      { apply Z2Nat.inj; ss. }
+      apply func_app with (f:=Int.repr) in H. rewrite Int.repr_signed in H. ss.
+    }
+    clarify.
+    rewrite Int.eq_true. des_ifs; repeat (Psimpl; des; ss; et).
+    step.
+  }
+  Fail rewrite bind_unwrapN. (*** <---------- TODO: FIXIT ***)
+  destruct (to_nat_opt (of_nat n0)) eqn:W; cbn; cycle 1.
+  { exfalso. unfold to_nat_opt in *. des_ifs. psimpl. unfold of_nat in *. rewrite Int.signed_repr in *; ss.
+    - xomega.
+    - generalize (Nat2Z.is_nonneg n0); i. generalize Int.min_signed_neg; i.
+      generalize (Int.signed_range i); i. subst x.
+      split; try xomega.
+      assert(Z.of_nat (S (S n0)) <= Int.max_signed).
+      { rewrite <- T. rewrite Z2Nat.id; ss. xomega. }
+      xomega.
+  }
+  assert(~Int.eq i Int.zero).
+  { ii. apply_all_once Int.same_if_eq. clarify. }
+  assert(~Int.eq i Int.one).
+  { ii. apply_all_once Int.same_if_eq. clarify. }
+  des_ifs_safe.
+  rewrite bind_ret_l.
+  rewrite bind_bind. rewrite ! bind_trigger.
+  (*** TODO: make lemma ***)
+  assert(SUCPRED: forall x y, x = S y <-> ((x - 1)%nat = y /\ (1 <= x)%nat)).
+  { clear - r. clear r.
+    split.
+    - ginduction x; ii; ss. clarify. split; try xomega. clear - y. ginduction y; ii; ss. et.
+    - ginduction x; ii; des; clarify; ss; try xomega. f_equal. rewrite Nat.sub_0_r. ss.
+  }
+  assert(U: of_nat n0 = Int.sub i (Int.repr 2)).
+  { unfold of_nat. subst x.
+    eapply SUCPRED in T; des.
+    eapply SUCPRED in T; des. ss. clarify.
+    (* rewrite <- Nat.sub_add_distr. ss. *)
+    rewrite Nat2Z.inj_sub; ss. rewrite Nat2Z.inj_sub; ss. rewrite <- Z.sub_add_distr; ss.
+    rewrite <- Int_sub_repr. f_equal. rewrite Z2Nat.id; ss. rewrite Int.repr_signed; ss.
+  }
+  rewrite <- U. step.
+  sii S. r in S. des_ifs_safe. des. clarify.
+  rewrite bind_bind.
+  (* unfold assume at 2. *)
+  Ltac step_assume := match goal with
+                      | |- context[assume ?P ;; _] =>
+                        (*** I want to unfold only the "first" assume.
+Maybe we should use notation instead, so that we can avoid this weird "unfold"? ***)
+                        first[
+                            unfold assume at 5|
+                            unfold assume at 4|
+                            unfold assume at 3|
+                            unfold assume at 2|
+                            unfold assume at 1|
+                            unfold assume at 0
+                          ];
+                        destruct (ClassicalDescription.excluded_middle_informative P); [
+                        |unfold triggerUB; rewrite bind_vis (*** <---------- this is counter-intuitive. Any good idea? ***);
+                         step]
+                      end
+  .
+  step_assume. des. clarify.
+  rewrite bind_ret_l.
+  rewrite bind_bind.
+  Ltac step_unwrapN := match goal with
+                       | |- context[unwrapN ?ox ;; _] =>
+                         (*** I want to unfold only the "first" assume.
+Maybe we should use notation instead, so that we can avoid this weird "unfold"? ***)
+                         first[
+                             unfold unwrapN at 5|
+                             unfold unwrapN at 4|
+                             unfold unwrapN at 3|
+                             unfold unwrapN at 2|
+                             unfold unwrapN at 1|
+                             unfold unwrapN at 0
+                           ];
+                         let name := fresh "T" in
+                         destruct ox eqn:name; cycle 1
+                       end
+  .
+  assert(V: of_nat (S n0) = Int.sub i (Int.repr 1)).
+  { unfold of_nat. subst x.
+    eapply SUCPRED in T; des.
+    eapply SUCPRED in T; des. ss. clarify.
+    rewrite Nat.sub_1_r. rewrite Nat.succ_pred; ss; cycle 1.
+    { intro X. rewrite X in *. inv T1. }
+    (* rewrite <- Nat.sub_add_distr. ss. *)
+    rewrite Nat2Z.inj_sub; ss.
+    rewrite <- Int_sub_repr. f_equal. rewrite Z2Nat.id; ss. rewrite Int.repr_signed; ss.
+  }
+  rewrite V.
+  step_unwrapN.
+  { exfalso. unfold to_nat_opt in *. des_ifs.
+    rewrite Int.signed_eq in *. des_sumbool. ss.
+    rewrite <- (@Int.repr_signed i) in g.
+    rewrite Int_sub_repr in *.
+    rewrite Int.signed_repr in *; ss.
+    - assert(Int.signed i = 0).
+      { xomega. }
+      ss.
+    - generalize (Int.signed_range i); i.
+      generalize Int.min_signed_neg; i. split; i; try lia.
+  }
+  cbn. rewrite bind_ret_l. rewrite ! bind_bind. rewrite ! bind_trigger. step.
+  sii S. r in S. des_ifs_safe; des; clarify.
+  rewrite bind_bind.
+  step_assume.
+  des; des_ifs_safe. rewrite bind_ret_l. rewrite bind_ret_l.
+  Ltac step_guaranteeK := match goal with
+                       | |- context[guaranteeK ?P ;; _] =>
+                         (*** I want to unfold only the "first" assume.
+Maybe we should use notation instead, so that we can avoid this weird "unfold"? ***)
+                         first[
+                             unfold guaranteeK at 5|
+                             unfold guaranteeK at 4|
+                             unfold guaranteeK at 3|
+                             unfold guaranteeK at 2|
+                             unfold guaranteeK at 1|
+                             unfold guaranteeK at 0
+                           ];
+                         destruct (ClassicalDescription.excluded_middle_informative P); cycle 1
+                       end
+  .
+  unfold guaranteeK. des_ifs; cycle 1.
+  { unfold NW in *. repeat (Psimpl; des; ss; et). }
+  des; clarify.
+  rewrite fib_nat_recurse.
+  unfold of_nat. rewrite Int_add_repr. rewrite Nat2Z.inj_add. step.
+Qed.
