demo/fib/Fib4.v
@@ -1,0 +1,119 @@
+Require Import CoqlibC Maps.
+Require Import ASTC Integers ValuesC EventsC MemoryC Globalenvs.
+Require Import Op Registers.
+Require Import sflib.
+Require Import SmallstepC.
+Require Export Simulation.
+Require Import Skeleton Mod ModSem.
+Require ClightC.
+Require Import Fib0.
+Require Import SIRmini.
+(* Require Import Clightdefs. *)
+
+Set Implicit Arguments.
+
+
+
+Definition owned_heap: Type := unit.
+Definition initial_owned_heap: SkEnv.t -> owned_heap := fun _ => tt.
+
+
+(* Definition to_nat (i: int): nat := Z.to_nat (Int.unsigned i). *)
+Definition to_nat (i: int): nat := Z.to_nat (Int.signed i).
+Definition of_nat (n: nat): int := Int.repr (Z.of_nat n).
+
+Definition to_nat_opt (i: int): option nat :=
+  if zle 0 (Int.signed i)
+  then Some (Z.to_nat (Int.signed i))
+  else None
+.
+
+Definition of_nat_opt (n: nat): option int :=
+  if zlt (Z.of_nat n) Int.modulus
+  then Some (Int.repr (Z.of_nat n))
+  else None
+.
+
+(* Goal forall x y (POS: Int.signed x + Int.signed y <= Int.max_signed) (POS: Int.signed x >= 0) (POS: Int.signed y >= 0), to_nat (Int.add x y) = Nat.add (to_nat x) (to_nat y). *)
+(* Proof. *)
+(*   i. unfold to_nat. *)
+(*   rewrite <- Z2Nat.inj_add; eauto with xomega. rewrite Int.add_signed. rewrite Int.signed_repr; ss. *)
+(*   split; try xomega. *)
+(*   - generalize Int.min_signed_neg; i. xomega. *)
+(* Qed. *)
+Fixpoint fib_nat (n: nat): nat :=
+  match n with
+  | 0%nat => 0%nat
+  | S n' =>
+    match n' with
+    | 0%nat => 1%nat
+    | S n'' => fib_nat n'' + fib_nat n'
+    end
+  end.
+
+(***
+precondition: exists n, vs = [Vint n]
+postcondition: OH unchanged && M unchanged && rv = of_nat (fib(n))
+***)
+
+(***
+Definition fib_spec fun_id :=
+ DECLARE fun_id
+  WITH n : Z
+  PRE  [ _n OF tint ]
+     PROP (0 <= n < 45) (* 50th term is too large to be a 32bit int *)
+     LOCAL (temp _n (Vint (Int.repr n)))
+     SEP ()
+  POST [ tint ]
+     PROP () LOCAL (temp ret_temp (Vint (Int.repr (fib_of_Z n))))
+     SEP ().
+***)
+
+Definition precond (vs: list val): option nat :=
+  match vs with
+  | [Vint n] => (to_nat_opt n)
+  | _ => None
+  end
+.
+Hint Unfold precond.
+Coercion is_some_coercion {X}: (option X) -> bool := is_some.
+
+Definition f_fib (oh0: owned_heap) (m0: mem) (vs: list val):
+  itree (E owned_heap) (owned_heap * (mem * val)) :=
+  tau;;
+  n <- (unwrapU (precond vs)) ;;
+  tau;;
+  tau;;
+  Ret (oh0, (m0, (Vint (of_nat (fib_nat n)))))
+.
+(*     else *)
+(*       if Nat.eqb n 0%nat *)
+(* Definition f_fib (oh0: owned_heap) (m0: mem) (vs: list val): *)
+(*   itree (E owned_heap) (owned_heap * (mem * val)) := *)
+(*   tau;; *)
+(*   match vs with *)
+(*   | [Vint n] => *)
+(*     if Int.eq n Int.zero *)
+(*     then Ret (oh0, (m0, (Vint Int.zero))) *)
+(*     else *)
+(*       if Int.eq n Int.one *)
+(*       then Ret (oh0, (m0, (Vint Int.one))) *)
+(*       else *)
+(*         (* guarantee (Int_le n Int.zero) ;; *) *)
+(*         guarantee True ;; *)
+(*         '(oh1, (m1, y1)) <- trigger (ICall _fib oh0 m0 [Vint (Int.sub n (Int.repr 2))]) ;; *)
+(*         (assume (fun _ => <<OH: oh0 = oh1>> /\ <<M: m0 = m1 >> /\ <<V: y1 = fib (Int.sub n (Int.repr 2))>>) tt) ;; *)
+
+(*         guarantee True ;; *)
+(*         '(oh2, (m2, y2)) <- trigger (ICall _fib oh1 m1 [Vint (Int.sub n (Int.repr 1))]) ;; *)
+(*         assume (<<OH: oh1 = oh2>> /\ <<M: m1 = m2 >> /\ <<V: y2 = fib (Int.sub n (Int.repr 1))>>) ;; *)
+(*         Ret (oh2, (m2, Val.add y1 y2)) *)
+(*   | _ => triggerUB *)
+(*   end *)
+(*   >>= *)
+(*   (fun '(ohr, (mr, vr)) => guarantee(<<OH: oh0 = ohr>> /\ <<M: m0 = mr>> /\ <<V: True>>) ;; Ret (ohr, (mr, vr))) *)
+(* . *)
+
+Definition prog: program owned_heap := (Maps.add _fib f_fib Maps.empty).
+
+Definition module: Mod.t := module (Fib0.module) prog "fib"%string initial_owned_heap.
